Attempt to write a hoare triplet for a heap write

SeparationLogic.v
@@ -4,86 +4,56 @@ Require Import Coq.Arith.EqNat.
 Require Import Coq.omega.Omega.
 Require Import Imp.
 Require Import Maps.
-
-(* Some house-keeping *)
-
-(* Redoing the definition for heap because we need some error checking on it *)
-Definition heap := partial_map nat.
-Definition empty_heap : heap := empty.
-
-Check valuation.
-
-(* The mixed embedding object language *)
-
-(* 
-   [res] gives the type of the value computed by [cmd] i.e, 
-   
-   cmd nat := heap -> (heap, (result of [cmd] of type [nat])).
-
-*)
-
-(* Needed for [Loop] *)
-Inductive looper a :=
-| Done (i : a)
-| Again (i : a).
+Require Import Hoare.
 
 
-Inductive cmd : Set -> Type :=
-| Return {res : Set}  : res -> cmd res
-(* Bind passes in the result of the command, [res'] as an argument to the the second [cmd], (the thing that comes up after [;])  *)                                   
-| Bind { res res' : Set} : cmd res' -> (res' -> cmd res) -> cmd res
-| Read : id -> cmd nat
-(* I guess, [cmd unit] would indicate that the type that [cmd] computes is nothing, as this is a [Write] op *)
-| Write : id -> nat -> cmd unit
-(* Takes in the number of indices to allocate in the heap as a [nat] *)
-| Alloc : (* number of contiguous memory spaces, 'n'*) nat -> cmd nat
-| Free : (* start, 'a' *) nat -> (* end, 'n' *) nat -> cmd unit
-(* [looper] checks if this the current condition of the loop is [Done] or [Again] *)
-| Loop {a : Set} : a -> (a -> cmd (looper a)) -> cmd a.
+(* The formula emp accepts only the empty heap *)
+Definition emp : Assertion :=
+  fun (h : heap) (_: valuation) => h = empty_heap. 
 
-Notation "x <- c1 ; c2" := (Bind c1 (fun x => c2)) (right associativity, at level 80).
+(* formula p -> a accepts only the heap whose only address is p, mapped to (aexp a) *)
+Definition ptoa (p : hid) (a : aexp) : Assertion :=
+  fun (h : heap) (v : valuation) =>
+    h = (update empty_heap p (aeval h v a)).
 
-(* Small step semantics *)
+(* Creating an existential quantifier that works for Assertions instead of Props.
+ * Ripping off a lot of stuff from First-order quantifiers section of : 
+ * https://coq.inria.fr/library/Coq.Init.Logic.html *)
+Definition ex_assert {A:Type} (P : A -> Assertion) : Assertion :=
+  fun h v => exists x, (P x) h v. 
 
-Fixpoint allocate (h : heap) (a n : nat) : heap  :=
-  match n with
-  | 0 => h
-  | S n' => allocate (update h (Id (a + n')) 0) a n'
-  end.
+(* definition of star *)
+Definition star (P Q : Assertion) : Assertion :=
+  fun (h : heap) (v : valuation) =>
+    exists h1, exists h2,
+        (* heap can be split into pieces /\ the split pieces are disjoint *) 
+        (h = h1 +++ h2) /\  h1 # h2 /\
+        (P h1 v) /\ (Q h2 v).
 
-Notation "h '[' a '|->' 'O(' n ')'  ']'" := (allocate h a n) (right associativity, at level 80).
+(* Some notations that will keep us in line with the frap book *)
+Notation "'exists' x .. y , p" := (ex_assert (fun x => .. (ex_assert (fun y => p)) ..)) : sep_scope.
+Notation " '*' p '|->' v" := (ptoa p v) (at level 50) : sep_scope.
+Notation " P * Q " := (star P Q) : sep_scope.
 
-Fixpoint deallocate (h: heap) (a n : nat) : heap :=
-  match n with
-  | 0 => h
-  | S n' => deallocate (remove h (Id a)) (a+1) n'
-  end.
+Delimit Scope sep_scope with sep.
+Local Open Scope sep_scope.
 
-Notation "h -- '[' a ',' 'a' '+' n ')' " := (deallocate h a n) (right associativity, at level 80). 
+Check (exists v, ( *(Id 10) |-> v))%sep.
 
-Inductive interp : forall {X : Set}, heap * cmd X -> heap * cmd X -> Prop  :=
-| BindStep : forall (res res' : Set) (c1 c1' : cmd res') (c2 : res' -> cmd res) (h h' : heap),
-    interp (h, c1) (h', c1') -> interp (h,  x <- c1; (c2 x)) (h', x <-c1'; (c2 x))
-| BindDone : forall (res res' : Set) (v : res') (c : res' -> cmd res)  (h : heap),
-    interp (h, (x <- Return v; c x)) (h, c v)
-| ReadStep : forall (a : id) (h : heap) (v : nat),
-    h a = Some v -> interp (h, Read a) (h, Return v)
-| WriteStep : forall (a : id) (h h' : heap) (v : nat) (u : unit),
-    (* https://coq.inria.fr/library/Coq.Init.Datatypes.html  *)
-    interp (h, Write a v) (h', Return u)
-| LoopStep : forall (acc : Set) (h : heap) (i : acc) (c : acc -> cmd (looper acc)),
-    interp (h, Loop i c) (h, x <- (c i); match x with
-                                         | Done _ a => Return a
-                                         | Again _ a => Loop a c
-                                         end)
-| AllocStep : forall (n a : nat) (h : heap),
-    (* make sure the range of allocated pieces stays between [a, a + n) *)
-    (forall i, i < n ->
-               (* if it does, make sure that those (a+n) adresses are unmapped *)
-               h (Id (a + i)) = None) ->
-    interp (h, Alloc n) (h[a |-> O(n)], Return a)
-| FreeStep : forall (n a : nat) (h : heap) (u : unit),
-    interp (h, Free a n) (h -- [a , a + n), Return u).
+(** ** Redoing Memory write *)
 
+(**
 
-(* 27th November 2016 *)
+      ------------------------------ (hoare_heap_write)
+      {{[*p] |-> v }} [*p] ::= v' {{ [*p] |-> v' }}
+ *)
+
+Lemma hoare_heap_write : forall (P : hid) (a : aexp),
+  {{ (exists v, *P |-> v)%sep }}
+    [*P] ::= a
+  {{ ( *P |-> a)%sep }}.
+Proof.
+  unfold hoare_triple.
+  intros P a h h' v v' H.  inversion H. subst. exists a.
+  
+  (* 27th November 2016 *)
